Paper/PreStar.thy
@@ -1,39 +1,37 @@
 section\<open>Applications\<close>
 text\<open>\label{sec:applications}\<close>
 
-text\<open>
-  The algorithm to compute \<open>pre\<^sup>*\<close> of a regular language can be used to construct
-  decision procedures for various different problems regarding context-free grammars.
-\<close>
-
 theory PreStar
-  imports Base.Algorithm "HOL.Finite_Set"
-begin \<comment>\<open>begin-theory Applications\<close>
+  imports Base.Pre_Star
+begin
 
-subsection\<open>Preliminaries\<close>
+(* TODO lemma "pre_star P (Lang_auto M) = Lang_auto (pre_star_auto P M)" *)
 
-text\<open>
-  The following code equations are necessary to make \texttt{nts\_syms} and \texttt{tms\_syms}
-  (and its dependents) automatically executable:
-\<close>
-(*
-lemma nts_syms_code[code]:
-  "nts_syms w = \<Union>((\<lambda>A. case A of Nt X \<Rightarrow> {X} | _ \<Rightarrow> {}) ` set w)"
-  by (auto simp: nts_syms_def split: sym.splits)
+text\<open>This theory turns @{const pre_star_auto} into executable decision procedures
+for different CFG problems. The methos: @{const pre_star_auto} is applied to different
+suitable automata/languages. This happens behind the scenes via code equations.\<close>
 
-lemma tms_syms_code[code]:
-  "tms_syms w = \<Union>((\<lambda>A. case A of Tm x \<Rightarrow> {x} | _ \<Rightarrow> {}) ` set w)"
-  by (auto simp: tms_syms_def split: sym.splits)
-*)
+text\<open>These lemmas link @{const pre_star} to different properties of context-free grammars:\<close>
+
+lemma pre_star_term:
+  "x \<in> pre_star P L \<longleftrightarrow> (\<exists>w. w \<in> L \<and> P \<turnstile> x \<Rightarrow>* w)"
+  unfolding pre_star_def by blast
+
+lemma pre_star_word:
+  "[Nt S] \<in> pre_star P (map Tm ` L) \<longleftrightarrow> (\<exists>w. w \<in> L \<and> w \<in> Lang P S)"
+  unfolding Lang_def pre_star_def by blast
+
+lemma pre_star_lang:
+  "Lang P S \<inter> L = {} \<longleftrightarrow> [(Nt S)] \<notin> pre_star P (map Tm ` L)"
+  using pre_star_word[where P=P] by blast
+
 subsection\<open>Derivability\<close>
 
-text\<open>
-  Particularly, a decision procedure for derivability can be constructed.
-\<close>
+text\<open>A decision procedure for derivability can be constructed.\<close>
 
-definition "is_derivable P \<alpha> \<beta> \<equiv> P \<turnstile> \<alpha> \<Rightarrow>* \<beta>"
+definition is_derivable :: "('n, 't) Prods \<Rightarrow> ('n, 't) syms \<Rightarrow> ('n, 't) syms \<Rightarrow> bool" where
+[simp]: "is_derivable P \<alpha> \<beta> = (P \<turnstile> \<alpha> \<Rightarrow>* \<beta>)"
 
-declare is_derivable_def[simp]
 declare is_derivable_def[symmetric, code_unfold]
 
 theorem pre_star_derivability:
@@ -42,14 +40,15 @@ theorem pre_star_derivability:
 
 lemma pre_star_derivability_code[code]:
   fixes P :: "('n, 't) prods"
-  shows "is_derivable (set P) \<alpha> \<beta> = (\<alpha> \<in> lang_nfa (prestar_nfa (set P) (nfa_word \<beta>)))"
+  shows "is_derivable (set P) \<alpha> \<beta> = (\<alpha> \<in> Lang_auto (pre_star_auto (set P) (word_auto \<beta>)))"
 proof -
-  define M where [simp]: "M \<equiv> nfa_word \<beta>"
-  have "lang_nfa (prestar_nfa (set P) M) = pre_star (set P) (lang_nfa M)"
-    by (intro prestar_nfa_correct; simp add: nfa_word_finite_trans)
+  define M where [simp]: "M \<equiv> word_auto \<beta>"
+  have "Lang_auto (pre_star_auto (set P) M) = pre_star (set P) (Lang_auto M)"
+    by (intro pre_star_auto_correct; simp add: word_auto_finite_lts)
   then show ?thesis
     using pre_star_derivability by force
 qed
+
 
 subsection\<open>Membership Problem\<close>
 
@@ -57,17 +56,21 @@ subsection\<open>Membership Problem\<close>
 lemma pre_star_membership[code_unfold]: "(w \<in> Lang P S) = (P \<turnstile> [Nt S] \<Rightarrow>* map Tm w)"
   by (simp add: Lang_def)
 
+
 subsection\<open>Nullable Variables\<close>
+
+definition is_nullable :: "('n, 't) Prods \<Rightarrow> 'n \<Rightarrow> bool" where
+  "is_nullable P X \<equiv> (P \<turnstile> [Nt X] \<Rightarrow>* [])"
 
 \<comment> \<open>Directly follows from derivability:\<close>
 lemma pre_star_nullable[code]: "is_nullable P X = (P \<turnstile> [Nt X] \<Rightarrow>* [])"
   by (simp add: is_nullable_def)
 
+
 subsection\<open>Emptiness Problem\<close>
 
-definition "is_empty P S \<equiv> Lang P S = {}"
-
-declare is_empty_def[simp]
+definition is_empty :: "('n, 't) Prods \<Rightarrow> 'n \<Rightarrow> bool" where
+[simp]:  "is_empty P S = (Lang P S = {})"
 
 lemma cfg_derives_Syms:
   assumes "P \<turnstile> \<alpha> \<Rightarrow>* \<beta>" and "set \<alpha> \<subseteq> Syms P"
@@ -84,7 +87,7 @@ next
     using step by simp
 qed
 
-lemma cfg_lang_univ: "P \<turnstile> [Nt X] \<Rightarrow>* map Tm \<beta> \<Longrightarrow> set \<beta> \<subseteq> Tms P"
+lemma cfg_Lang_univ: "P \<turnstile> [Nt X] \<Rightarrow>* map Tm \<beta> \<Longrightarrow> set \<beta> \<subseteq> Tms P"
 proof -
   assume "P \<turnstile> [Nt X] \<Rightarrow>* map Tm \<beta>"
   moreover have "Nt X \<in> Syms P"
@@ -111,10 +114,10 @@ qed
 lemma finite_Tms: "finite P \<Longrightarrow> finite (Tms P)"
   unfolding Tms_def by (rule finite_Union; auto simp: finite_tms_syms)
 
-definition pre_star_emptiness_nfa :: "('n, 't) Prods \<Rightarrow> (unit, ('n, 't) sym) nfa" where
-  "pre_star_emptiness_nfa P \<equiv>
+definition pre_star_emptiness_auto :: "('n, 't) Prods \<Rightarrow> (unit, ('n, 't) sym) auto" where
+  "pre_star_emptiness_auto P \<equiv>
     let T = Tm ` \<Union>((\<lambda>A. case A of Nt X \<Rightarrow> {} | Tm x \<Rightarrow> {x}) ` \<Union>(set ` snd ` P)) :: ('n, 't) sym set in
-    \<lparr> transitions = {()} \<times> T \<times> {()}, start = (), finals = {()} \<rparr>"
+    \<lparr> auto.lts = {()} \<times> T \<times> {()}, start = (), finals = {()} \<rparr>"
 
 theorem pre_star_emptiness:
   fixes P :: "('n, 't) Prods"
@@ -123,9 +126,9 @@ proof -
   have "Lang P S = {} \<longleftrightarrow> (\<nexists>w. P \<turnstile> [Nt S] \<Rightarrow>* map Tm w)"
     by (simp add: Lang_def)
   also have "... \<longleftrightarrow> (\<nexists>w. P \<turnstile> [Nt S] \<Rightarrow>* map Tm w \<and> set w \<subseteq> Tms P)"
-    using cfg_lang_univ by fast
+    using cfg_Lang_univ by fast
   also have "... \<longleftrightarrow> (\<nexists>w. P \<turnstile> [Nt S] \<Rightarrow>* w \<and> set w \<subseteq> Tm ` Tms P)"
-    by (smt (verit, best) cfg_lang_univ ex_map_conv imageE image_mono list.set_map subset_iff)
+    by (smt (verit, best) cfg_Lang_univ ex_map_conv imageE image_mono list.set_map subset_iff)
   also have "... \<longleftrightarrow> [Nt S] \<notin> pre_star P {w. set w \<subseteq> Tm ` Tms P}"
     unfolding pre_star_def by blast
   finally show ?thesis .
@@ -133,23 +136,32 @@ qed
 
 lemma pre_star_emptiness_code[code]:
   fixes P :: "('n, 't) prods"
-  shows "is_empty (set P) S = ([Nt S] \<notin> lang_nfa (prestar_nfa (set P) (nfa_univ (Tm ` Tms (set P)))))"
+  shows "is_empty (set P) S = ([Nt S] \<notin> Lang_auto (pre_star_auto (set P) (auto_univ (Tm ` Tms (set P)))))"
 proof -
-  define M :: "(unit, ('n, 't) sym) nfa" where [simp]: "M \<equiv> nfa_univ (Tm ` Tms (set P))"
+  define M :: "(unit, ('n, 't) sym) auto" where [simp]: "M \<equiv> auto_univ (Tm ` Tms (set P))"
   have "finite (Tm ` Tms (set P))"
     using finite_Tms by blast
-  then have "lang_nfa (prestar_nfa (set P) M) = pre_star (set P) (lang_nfa M)"
-    by (intro prestar_nfa_correct; auto simp: nfa_univ_def intro: nfa_univ_trans_fin)
+  then have "Lang_auto (pre_star_auto (set P) M) = pre_star (set P) (Lang_auto M)"
+    by (intro pre_star_auto_correct; auto simp: auto_univ_def intro: loop_lts_fin)
   then show ?thesis
-    using pre_star_emptiness unfolding M_def nfa_univ_lang by fastforce
+    using pre_star_emptiness unfolding M_def auto_univ_lang by fastforce
 qed
+
 
 subsection\<open>Useless Variables\<close>
 
-definition pre_star_reachable_nfa :: "('n, 't) Prods \<Rightarrow> 'n \<Rightarrow> (nat, ('n, 't) sym) nfa" where
-  "pre_star_reachable_nfa P X \<equiv> (
+definition is_reachable_from :: "('n, 't) Prods \<Rightarrow> 'n \<Rightarrow> 'n \<Rightarrow> bool"
+    ("(2_ \<turnstile>/ (_/ \<Rightarrow>\<^sup>? / _))" [50, 0, 50] 50) where
+  "(P \<turnstile> X \<Rightarrow>\<^sup>? Y) \<equiv> (\<exists>\<alpha> \<beta>. P \<turnstile> [Nt X] \<Rightarrow>* (\<alpha>@[Nt Y]@\<beta>))"
+
+\<comment>\<open>\<open>X \<in> V\<close> is useful, iff \<open>V\<close> can be reached from \<open>S\<close> and it is productive:\<close>
+definition is_useful :: "('n, 't) Prods \<Rightarrow> 'n \<Rightarrow> 'n \<Rightarrow> bool" where
+  "is_useful P S X \<equiv> (P \<turnstile> S \<Rightarrow>\<^sup>? X) \<and> Lang P X \<noteq> {}"
+
+definition pre_star_reachable_auto :: "('n, 't) Prods \<Rightarrow> 'n \<Rightarrow> (nat, ('n, 't) sym) auto" where
+  "pre_star_reachable_auto P X \<equiv> (
     let T = \<Union>(set ` snd ` P) in
-    \<lparr> transitions = ({0} \<times> T \<times> {0}) \<union> ({1} \<times> T \<times> {1}) \<union> {(0, Nt X, 1)}, start = 0, finals = {1} \<rparr>
+    \<lparr> auto.lts = ({0} \<times> T \<times> {0}) \<union> ({1} \<times> T \<times> {1}) \<union> {(0, Nt X, 1)}, start = 0, finals = {1} \<rparr>
   )"
 
 theorem pre_star_reachable:
@@ -178,44 +190,17 @@ qed
 
 lemma pre_star_reachable_code[code]:
   fixes P :: "('n, 't) prods"
-  shows "((set P) \<turnstile> S \<Rightarrow>\<^sup>? X) = ([Nt S] \<in> lang_nfa (prestar_nfa (set P) (nfa_fixc_ps (Nt X) (Syms (set P)))))"
+  shows "(set P \<turnstile> S \<Rightarrow>\<^sup>? X) = ([Nt S] \<in> Lang_auto (pre_star_auto (set P) (cps_auto (Nt X) (Syms (set P)))))"
 proof -
-  define M :: "(nat, ('n, 't) sym) nfa" where [simp]: "M \<equiv> nfa_fixc_ps (Nt X) (Syms (set P))"
+  define M :: "(nat, ('n, 't) sym) auto" where [simp]: "M \<equiv> cps_auto (Nt X) (Syms (set P))"
   have "finite (Syms (set P))"
     unfolding Syms_def by fast
-  then have "lang_nfa (prestar_nfa (set P) M) = pre_star (set P) (lang_nfa M)"
-    by (intro prestar_nfa_correct; auto simp: nfa_fixc_ps_def intro: nfa_fixc_ps_trans_fin)
+  then have "Lang_auto (pre_star_auto (set P) M) = pre_star (set P) (Lang_auto M)"
+    by (intro pre_star_auto_correct; auto simp: cps_auto_def intro: pcs_lts_fin)
   then show ?thesis
-    using pre_star_reachable unfolding M_def nfa_fixc_ps_lang by fastforce
+    using pre_star_reachable unfolding M_def cps_auto_lang by fastforce
 qed
 
-theorem pre_star_productive:
-  fixes P :: "('n, 't) Prods"
-  shows "is_productive P X \<longleftrightarrow> [(Nt X)] \<in> pre_star P {w. set w \<subseteq> Tm ` Tms P}"
-proof -
-  have "is_productive P X \<longleftrightarrow> (\<exists>w. P \<turnstile> [Nt X] \<Rightarrow>* map Tm w)"
-    by (simp add: is_productive_def)
-  also have "... \<longleftrightarrow> (\<exists>w. P \<turnstile> [Nt X] \<Rightarrow>* map Tm w \<and> set w \<subseteq> Tms P)"
-    using cfg_lang_univ by fast
-  also have "... \<longleftrightarrow> (\<exists>w. P \<turnstile> [Nt X] \<Rightarrow>* w \<and> set w \<subseteq> Tm ` Tms P)"
-    by (smt (verit, best) cfg_lang_univ ex_map_conv imageE image_mono list.set_map subset_iff)
-  also have "... \<longleftrightarrow> [Nt X] \<in> pre_star P {w. set w \<subseteq> Tm ` Tms P}"
-    unfolding pre_star_def by blast
-  finally show ?thesis .
-qed
-
-lemma pre_star_productive_code[code]:
-  fixes P :: "('n, 't) prods"
-  shows "is_productive (set P) X = ([Nt X] \<in> lang_nfa (prestar_nfa (set P) (nfa_univ (Tm ` Tms (set P)))))"
-proof -
-  define M :: "(unit, ('n, 't) sym) nfa" where [simp]: "M \<equiv> nfa_univ (Tm ` Tms (set P))"
-  have "finite (Tm ` Tms (set P))"
-    using finite_Tms by blast
-  then have "lang_nfa (prestar_nfa (set P) M) = pre_star (set P) (lang_nfa M)"
-    by (intro prestar_nfa_correct; auto simp: nfa_univ_def intro: nfa_univ_trans_fin)
-  then show ?thesis
-    using pre_star_productive unfolding M_def nfa_univ_lang by fastforce
-qed
 
 subsection\<open>Disjointness and Subset Problem\<close>
 
@@ -230,4 +215,4 @@ proof -
     by (simp add: pre_star_disjointness)
 qed
 
-end \<comment>\<open>end-theory Applications\<close>
+end
